Begin to adapt backend pointers
Checkpoint on ValType refactoring for the new capability backend. Very
similar to CompCert standard values, refactoring the pointer part of the
definitions.

Proofs are very similar to those for standard pointers, sometimes with
added case analysis on the shape of the pointers (stack or heap). The
ValType specs line up better with this instance and all problematic
lemmas in the previous instance, except one, are proved right away.

cheririscV/OCapValues.v
@@ -20,6 +20,7 @@ Require Import Coqlib.
 Require Import CapAST.
 Require Import Integers.
 Require Import Floats.
+Require Import ValType.
 
 Definition seal := ptrofs.
 
@@ -346,9 +347,363 @@ Definition incr_addr_stk (v: occap) (ofs: Z) : option occap :=
   | _ => None
   end.
 
-Inductive pointer: Type :=
-| heap_ptr: ptrofs -> pointer
-| stack_ptr: ptrofs -> pointer.
+Module Ptr : VAL.
+
+(*
+Error:
+The kernel does not recognize yet that a parameter can be instantiated by an inductive type. Hint: you can rename the inductive type and give a definition to map the old name to the new name.
+*)
+Inductive pointer': Type :=
+| heap_ptr: ptrofs -> pointer'
+| stack_ptr: ptrofs -> pointer'.
+
+Let pointer := pointer'.
+
+Theorem eq_dec_pointer: forall (p1 p2: pointer), {p1 = p2} + {~ p1 = p2}.
+Proof.
+  decide equality.
+  - now apply Ptrofs.eq_dec.
+  - now apply Ptrofs.eq_dec.
+Qed.
+
+Definition pointer_arith (f: ptrofs -> ptrofs -> ptrofs) (ptr1: pointer) (ofs: ptrofs): pointer :=
+  match ptr1 with
+  | heap_ptr ofs1 => heap_ptr (f ofs1 ofs)
+  | stack_ptr ofs1 => stack_ptr (f ofs1 ofs)
+  end.
+
+Definition pointer_add (ptr: pointer) (n2: ptrofs) : option pointer :=
+  if Archi.ptr64 then None else Some (pointer_arith Ptrofs.add ptr n2).
+
+Definition pointer_sub (ptr: pointer) (n2: ptrofs) : option pointer :=
+  if Archi.ptr64 then None else Some (pointer_arith Ptrofs.sub ptr n2).
+
+Definition pointer_pointer_sub (ptr1 ptr2: pointer) : option ptrofs :=
+  match ptr1, ptr2 with
+  | heap_ptr ofs1, heap_ptr ofs2
+  | stack_ptr ofs1, stack_ptr ofs2 =>
+      if Archi.ptr64 then None else
+        Some (Ptrofs.sub ofs1 ofs2)
+  | _, _ => None
+  end.
+
+(** Comparisons *)
+
+Section COMPARISONS.
+
+(* Variable valid_ptr: Z -> bool. *)
+(* TODO Check interface *)
+Definition valid_ptr: Z -> bool := fun _ => true.
+Let weak_valid_ptr (ofs: Z) := valid_ptr ofs || valid_ptr (ofs - 1).
+
+Definition pointer_pointer_cmpu (diff_blocks: option bool) (c: comparison) (ptr1 ptr2: pointer) : option bool :=
+  match ptr1, ptr2 with
+  | stack_ptr ofs1, stack_ptr ofs2
+  | heap_ptr ofs1, heap_ptr ofs2 =>
+      if Archi.ptr64 then None else
+        if weak_valid_ptr (Ptrofs.unsigned (ofs1))
+           && weak_valid_ptr (Ptrofs.unsigned (ofs2))
+        then Some (Ptrofs.cmpu c (ofs1) (ofs2))
+        else None
+  | _, _ => None
+  end.
+
+End COMPARISONS.
+
+Theorem pointer_add_assoc_int:
+  forall ptr i1 i2,
+    Archi.ptr64 = false ->
+    pointer_add ptr (Ptrofs.of_int (Int.add i1 i2)) =
+      match pointer_add ptr (Ptrofs.of_int i1) with
+      | Some ptr' => pointer_add ptr' (Ptrofs.of_int i2)
+      | None => None
+      end.
+Proof.
+  intros ptr i1 i2 ARCHI.
+  unfold pointer_add, pointer_arith.
+  rewrite ARCHI.
+  destruct ptr as [ofs | ofs].
+  - rewrite Ptrofs.add_assoc.
+    erewrite Ptrofs.agree32_of_int_eq; [reflexivity |].
+    apply Ptrofs.agree32_add;
+      [assumption | |];
+      now apply Ptrofs.agree32_of_int.
+  - rewrite Ptrofs.add_assoc.
+    erewrite Ptrofs.agree32_of_int_eq; [reflexivity |].
+    apply Ptrofs.agree32_add;
+      [assumption | |];
+      now apply Ptrofs.agree32_of_int.
+Qed.
+
+Theorem pointer_add_assoc_long:
+  forall ptr i1 i2,
+    Archi.ptr64 = true ->
+    pointer_add ptr (Ptrofs.of_int64 (Int64.add i1 i2)) =
+      match pointer_add ptr (Ptrofs.of_int64 i1) with
+      | Some ptr' => pointer_add ptr' (Ptrofs.of_int64 i2)
+      | None => None
+      end.
+Proof.
+  intros ptr i1 i2 ARCHI.
+  unfold pointer_add.
+  rewrite ARCHI.
+  reflexivity.
+Qed.
+
+Theorem pointer_add_commut:
+  forall ptr i1 i2,
+    match pointer_add ptr i1 with
+    | Some ptr' => pointer_add ptr' i2
+    | None => None
+    end =
+    match pointer_add ptr i2 with
+    | Some ptr' => pointer_add ptr' i1
+    | None => None
+    end.
+Proof.
+  intros ptr i1 i2.
+  unfold pointer_add, pointer_arith.
+  destruct Archi.ptr64 eqn:ARCHI; [reflexivity |].
+  destruct ptr as [ofs | ofs].
+  - rewrite !Ptrofs.add_assoc.
+    now rewrite (Ptrofs.add_commut i2 i1).
+  - rewrite !Ptrofs.add_assoc.
+    now rewrite (Ptrofs.add_commut i2 i1).
+Qed.
+
+Theorem pointer_add_sub_l:
+  forall ptr i1 i2,
+    match pointer_add ptr i1 with
+    | Some ptr' => pointer_sub ptr' i2
+    | None => None
+    end =
+    match pointer_sub ptr i2 with
+    | Some ptr' => pointer_add ptr' i1
+    | None => None
+    end.
+  intros ptr i1 i2.
+  unfold pointer_add, pointer_sub, pointer_arith.
+  destruct Archi.ptr64 eqn:ARCHI; [reflexivity |].
+  destruct ptr as [ofs | ofs].
+  - now rewrite Ptrofs.sub_add_l.
+  - now rewrite Ptrofs.sub_add_l.
+Qed.
+
+Theorem pointer_pointer_add_sub_l:
+  forall ptr i1 i2,
+    match pointer_add ptr i1 with
+    | Some ptr' => pointer_pointer_sub ptr' i2
+    | None => None
+    end =
+    match pointer_pointer_sub ptr i2 with
+    | Some ptrofs => Some (Ptrofs.add i1 ptrofs)
+    | None => None
+    end.
+Proof.
+  intros ptr1 i ptr2.
+  unfold pointer_add, pointer_pointer_sub, pointer_arith.
+  destruct Archi.ptr64 eqn:ARCHI;
+    [destruct ptr1; destruct ptr2; reflexivity |].
+  destruct ptr1 as [ofs1 | ofs1]; destruct ptr2 as [ofs2 | ofs2].
+  - rewrite Ptrofs.sub_add_l.
+    now rewrite Ptrofs.add_commut.
+  - reflexivity.
+  - reflexivity.
+  - rewrite Ptrofs.sub_add_l.
+    now rewrite Ptrofs.add_commut.
+Qed.
+
+Theorem pointer_add_sub_neg_int:
+  forall p y,
+    pointer_sub p (Ptrofs.of_int y) = pointer_add p (Ptrofs.of_int (Int.neg y)).
+Proof.
+  intros ptr y.
+  unfold pointer_sub, pointer_add, pointer_arith.
+  destruct Archi.ptr64 eqn:ARCHI; [reflexivity |].
+  f_equal. f_equal.
+  destruct ptr as [ofs | ofs].
+  - erewrite (Ptrofs.agree32_of_int_eq _ (Int.neg y)).
+    + now rewrite Ptrofs.sub_add_opp.
+    + apply Ptrofs.agree32_neg; [assumption |].
+      now apply Ptrofs.agree32_of_int.
+  - erewrite (Ptrofs.agree32_of_int_eq _ (Int.neg y)).
+    + now rewrite Ptrofs.sub_add_opp.
+    + apply Ptrofs.agree32_neg; [assumption |].
+      now apply Ptrofs.agree32_of_int.
+Qed.
+
+Theorem pointer_add_sub_neg_long:
+  forall p y,
+    pointer_sub p (Ptrofs.of_int64 y) = pointer_add p (Ptrofs.of_int64 (Int64.neg y)).
+Proof.
+  intros ptr y.
+  unfold pointer_sub, pointer_add, pointer_arith.
+  destruct Archi.ptr64 eqn:ARCHI; [reflexivity |].
+  destruct ptr as [ofs | ofs].
+  (* this one's a bit trickier *)
+Admitted.
+
+Definition offset_pointer (ptr: pointer) (delta: ptrofs) : option pointer :=
+  Some (pointer_arith Ptrofs.add ptr delta).
+
+Theorem offset_pointer_zero:
+  forall p, offset_pointer p (Ptrofs.zero) = Some p.
+Proof.
+  intros ptr.
+  unfold offset_pointer, pointer_arith.
+  destruct ptr as [ofs | ofs].
+  - now rewrite Ptrofs.add_zero.
+  - now rewrite Ptrofs.add_zero.
+Qed.
+
+(* TODO *)
+Definition normalize_pointer (p: pointer) (t: AST.captyp) : bool :=
+  match t with
+  | AST.CTint | AST.CTany32 => negb Archi.ptr64
+  | AST.CTlong => Archi.ptr64
+  | AST.CTany64 => true
+  | AST.CTany128 => true
+  | _ => false (* "new" fallback *)
+  end.
+
+(* TODO *)
+Definition pointer_load_result (chunk: AST.cap_memory_chunk) (p: pointer) : bool :=
+  match chunk with
+  | AST.CMint32 => negb Archi.ptr64
+  | AST.CMint64 => Archi.ptr64
+  | AST.CMany32 => negb Archi.ptr64
+  | AST.CMany64 => true
+  | AST.CMany128 => true
+  | _ => false (* "new" fallback *)
+  end.
+
+(* TODO *)
+Definition has_type_pointer (_: pointer) (t: AST.captyp) : Prop := (* remove parameter? *)
+  match t with
+  | AST.CTint => Archi.ptr64 = false
+  | AST.CTlong => Archi.ptr64 = true
+  | AST.CTany64 => True
+  | AST.CTany32 => Archi.ptr64 = false
+  | AST.CTany128 => True
+  | _ => False (* "new" fallback *)
+  end.
+
+Theorem has_type_pointer_dec:
+  forall p t, {has_type_pointer p t} + {~ has_type_pointer p t}.
+Proof.
+  unfold has_type_pointer.
+  intros _ []; auto; decide equality.
+Qed.
+
+Theorem has_subtype_pointer:
+  forall ty1 ty2 v,
+    AST.subtype ty1 ty2 = true -> has_type_pointer v ty1 -> has_type_pointer v ty2.
+Proof.
+  intros [] [] [|] SUB PTR;
+    easy.
+Qed.
+
+Theorem has_type_pointer_int:
+  forall p, has_type_pointer p AST.CTint -> Archi.ptr64 = false.
+Proof.
+  simpl. now auto.
+Qed.
+
+Theorem has_type_pointer_long:
+  forall p, has_type_pointer p AST.CTlong -> Archi.ptr64 = true.
+Proof.
+  simpl. now auto.
+Qed.
+
+Theorem has_type_pointer_cap64:
+  forall p, has_type_pointer p AST.CTcap64 -> Archi.ptr64 = false.
+Proof.
+  simpl. now auto.
+Qed.
+
+Theorem has_type_pointer_cap128:
+  forall p, has_type_pointer p AST.CTcap128 -> Archi.ptr64 = true.
+Proof.
+  simpl. now auto.
+Qed.
+
+Theorem has_type_pointer_cases:
+  forall p ty,
+    has_type_pointer p ty ->
+    ty = AST.CTint \/ ty = AST.CTlong \/ ty = AST.CTcap64 \/ ty = AST.CTcap128.
+Proof.
+  intros [|] []; try now auto.
+  (* doesn't work *)
+Abort.
+
+Theorem has_type_pointer_load_result:
+  forall p chunk,
+    pointer_load_result chunk p = true ->
+    has_type_pointer p (type_of_cap_chunk chunk).
+Proof.
+  intros ptr []; try easy.
+  - simpl. now apply negb_true_iff.
+  - simpl. now apply negb_true_iff.
+Qed.
+
+Theorem load_result_has_type_pointer:
+  forall p ty,
+    has_type_pointer p ty ->
+    pointer_load_result (chunk_of_captype ty) p = true.
+Proof.
+  intros ptr []; try easy.
+  - simpl. now apply negb_true_iff.
+  - simpl. now apply negb_true_iff.
+Qed.
+
+Theorem normalize_has_type_pointer:
+  forall p ty,
+    normalize_pointer p ty = true ->
+    has_type_pointer p ty.
+Proof.
+  intros ptr []; try easy.
+  - simpl. now apply negb_true_iff.
+  - simpl. now apply negb_true_iff.
+Qed.
+
+Theorem has_type_pointer_normalize:
+  forall p ty,
+    has_type_pointer p ty ->
+    normalize_pointer p ty = true.
+Proof.
+  intros ptr []; try easy.
+  - simpl. now apply negb_true_iff.
+  - simpl. now apply negb_true_iff.
+Qed.
+
+Theorem normalize_any:
+  forall p, normalize_pointer p AST.CTany128 = true.
+Proof.
+  reflexivity.
+Qed.
+
+Inductive val: Type :=
+| Vundef: val
+| Vint: int -> val
+| Vlong: int64 -> val
+| Vfloat: float -> val
+| Vsingle: float32 -> val
+| Vptr: pointer -> val.
+
+Definition Vzero: val := Vint Int.zero.
+Definition Vone: val := Vint Int.one.
+Definition Vmone: val := Vint Int.mone.
+
+Definition Vtrue: val := Vint Int.one.
+Definition Vfalse: val := Vint Int.zero.
+
+Definition Vnullptr :=
+  if Archi.ptr64 then Vlong Int64.zero else Vint Int.zero.
+
+Definition Vptrofs (n: ptrofs) :=
+  if Archi.ptr64 then Vlong (Ptrofs.to_int64 n) else Vint (Ptrofs.to_int n).
+
+End Ptr.
 
 Definition pointer_ofs (ptr: pointer): ptrofs :=
   match ptr with
@@ -728,6 +1083,7 @@ Definition pointer_arith (f: ptrofs -> ptrofs -> ptrofs) (ptr1: pointer) (ofs: p
   | heap_ptr ofs1 => heap_ptr (f ofs1 ofs)
   | stack_ptr ofs1 => stack_ptr (f ofs1 ofs)
   end.
+(* TODO: currently copied in Ptr above *)
 
 Definition add (v1 v2: ocval): ocval :=
   match v1, v2 with
